\documentclass[11pt]{amsart}
\usepackage{mathtools}
\usepackage{enumitem}

\begin{document}

\begin{enumerate}[label=\Alph*)]

	\begin{enumerate}[label=\roman)*]
		\item $\sum_{i=1}^{n} i^2 = \frac{n(n+1)(2n+1)}{6}$

		\begin{proof}
			Suppose $n=1$, we have $1^2 = \frac{1(1+1)(2+1)}{6}$ \\

			Assume that for some positive integer $k, \sum_{i=1}^{k} i = \frac{k(k+1)(2k+1)}{6}$ \\

			\begin{align*}
				\sum_{i=1}^{k+1} i^2 &= \sum_{i=1}^{k} i^2 + (k+1)^2 = \frac{k(k+1)(2k+1)}{6} + (k+1)^2 \\
				&= (k+1)\left[\frac{k(2k+1)+6(k+1)}{6}\right] = (k+1)\left[\frac{2k^3 +7k + 6}{6}\right] \\
				&= \frac{(k+1)(k+2)(2k+3)}{6},
			\end{align*}

			giving us the desired result. By the Principle of Mathematical Induction,

			\[
				\sum_{i=1}^{n} i^2 = \frac{n(n+1)(2n+1)}{6}
			\]
		\end{proof}

		\item $1^3 + \cdots \, + n^3 = \left(1 + \dots + n\right)^2$

		\bigskip

		Do note that $1^3 + \cdots \, + n^3$ is the same as $\sum_{i=1}^n i^3$ and that\\

		$\left(1 + \cdots + n\right)^2 = \left(\sum_{i=1}^n i\right)^2 = \left(\frac{n(n+1)}{2}\right)^2$
		$= \frac{n^2(n+1)^2}{4}$ \\

		\medskip

		So we can simplify the problem into;

		\medskip

		$\sum_{i=1}^n i^3 = \frac{n^2(n+1)^2}{4}$ \\

		\begin{proof}
			Let $n=1$, then $1^3 = \frac{1^2 \, (1+1)^2}{4}$. Hence the proposition is true.\\

			Now assume that, $\sum_{i=1}^{k} i^3 = \frac{k^2\,(k+1)^2}{4}$ is true for some positive integer $k$.

			Then,\\

			\begin{align*}
				\sum_{i=1}^{k+1} i^3 &= \sum_{i=1}^{k} i^3 + (k+1)^3 = \frac{k^2 (k+1)^2}{4} + (k+1)^3 \\
						     &= (k+1)^2 \left[\frac{k^2 + 4(k+1)}{4}\right] = (k+1)^2\left[\frac{k^2 + 4k + 4}{4}\right]\\
				&= \frac{(k+1)^2/,(k+2)^2}{2}
			\end{align*}

			By the principle of induction, the formula holds for all positive integers $n$.
	\end{proof}


%\begin{align}
%	\sum_{i=1}^n (2i-1) = 1 + 3 + 5 + \cdots (2i-1)
%\end{align}
%
%\end{enumerate}
\end{document}
